Soundness.v
@@ -1,52 +1,12 @@
+From Coq Require Import Arith.Arith.
+From Coq Require Import Lia.
+From Coq Require Strings.String.
+
 From Elo Require Import Array.
 From Elo Require Import Map.
 From Elo Require Import Core.
-
-Inductive well_behaved_locations (m : mem) : tm -> Prop :=
-  | wbl_unit :
-    well_behaved_locations m TM_Unit 
-
-  | wbl_num : forall n,
-    well_behaved_locations m (TM_Num n)
-
-  | wbl_loc : forall T ad,
-    empty |-- (getTM m ad) is T ->
-    well_behaved_locations m (TM_Loc T ad)
-
-  | wbl_new : forall T t,
-    well_behaved_locations m t ->
-    well_behaved_locations m (TM_New T t) 
-
-  | wbl_load : forall t,
-    well_behaved_locations m t ->
-    well_behaved_locations m (TM_Load t) 
-
-  | wbl_asg : forall t1 t2,
-    well_behaved_locations m t1 ->
-    well_behaved_locations m t2 ->
-    well_behaved_locations m (TM_Asg t1 t2) 
-
-  | wbl_id : forall id,
-    well_behaved_locations m (TM_Id id)
-
-  | wbl_fun : forall x Tx t,
-    well_behaved_locations m t ->
-    well_behaved_locations m (TM_Fun x Tx t) 
-
-  | wbl_call : forall t1 t2,
-    well_behaved_locations m t1 ->
-    well_behaved_locations m t2 ->
-    well_behaved_locations m (TM_Call t1 t2) 
-
-  | wbl_seq : forall t1 t2,
-    well_behaved_locations m t1 ->
-    well_behaved_locations m t2 ->
-    well_behaved_locations m (TM_Seq t1 t2) 
-
-  | wbl_spawn : forall t,
-    well_behaved_locations m t ->
-    well_behaved_locations m (TM_Spawn t) 
-  .
+From Elo Require Import Access.
+From Elo Require Import WBA.
 
 Lemma context_weakening : forall Gamma Gamma' t T,
   Gamma includes Gamma' ->
@@ -64,6 +24,112 @@ Lemma context_weakening_empty : forall Gamma t T,
 Proof.
   intros. eapply (context_weakening _ empty); trivial. discriminate.
 Qed.
+
+(* ------------------------------------------------------------------------- *)
+(* ------------------------------------------------------------------------- *)
+(* ------------------------------------------------------------------------- *)
+
+Inductive well_behaved_references (m : mem) : tm -> Prop :=
+  | wbr_unit :
+    well_behaved_references m <{ unit }> 
+
+  | wbr_num : forall n,
+    well_behaved_references m <{ N n }>
+
+  | wbr_refM : forall T ad,
+    empty |-- (getTM m ad) is T ->
+    well_behaved_references m <{ &ad: (&m T) }>
+
+  | wbr_refI : forall T ad,
+    empty |-- (getTM m ad) is T ->
+    well_behaved_references m <{ &ad: (&i T) }>
+
+  | wbr_new : forall T t,
+    well_behaved_references m t ->
+    well_behaved_references m <{ new T t }> 
+
+  | wbr_load : forall t,
+    well_behaved_references m t ->
+    well_behaved_references m <{ *t }> 
+
+  | wbr_asg : forall t1 t2,
+    well_behaved_references m t1 ->
+    well_behaved_references m t2 ->
+    well_behaved_references m <{ t1 = t2 }> 
+
+  | wbr_id : forall x,
+    well_behaved_references m <{ ID x }>
+
+  | wbr_fun : forall x Tx t,
+    well_behaved_references m t ->
+    well_behaved_references m <{ fun x: Tx -> t }>
+
+  | wbr_call : forall t1 t2,
+    well_behaved_references m t1 ->
+    well_behaved_references m t2 ->
+    well_behaved_references m <{ t1 t2 }> 
+
+  | wbr_seq : forall t1 t2,
+    well_behaved_references m t1 ->
+    well_behaved_references m t2 ->
+    well_behaved_references m <{ t1; t2 }> 
+  .
+
+Lemma wbr_subst : forall m x Tx t v,
+  well_behaved_references m v ->
+  well_behaved_references m <{ fun x: Tx -> t }> ->
+  well_behaved_references m ([x := v] t).
+Proof.
+  intros * ? H. 
+  assert (H' : well_behaved_references m t). { inversion H. trivial. } clear H.
+  induction t; simpl; try (destruct String.string_dec);
+  inversion H'; eauto using well_behaved_references.
+Qed.
+
+Lemma wbr_mem_add : forall m t v, 
+  well_behaved_access m t ->
+  well_behaved_references m t ->
+  well_behaved_references (add m v) t.
+Proof.
+  intros * Hwba Hwbr. induction t; eauto using well_behaved_references;
+  inversion_clear Hwbr; subst; try (destruct_wba);
+  eauto using well_behaved_references;
+  try (eapply wbr_refM || eapply wbr_refI);
+  decompose sum (lt_eq_lt_dec (length m) n); subst;
+  solve [ rewrite (get_add_gt TM_Unit); trivial;
+          specialize (Hwba _ (access_loc _ _ _)); lia
+        | rewrite (get_add_eq TM_Unit); trivial;
+          specialize (Hwba _ (access_loc _ _ _)); lia
+        | rewrite (get_add_lt TM_Unit); trivial
+        ].
+Qed.
+
+Lemma wbr_preservation : forall m m' t t' eff T,
+  empty |-- t is T ->
+  well_behaved_access m t ->
+  well_behaved_references m t ->
+  m / t ==[eff]==> m' / t' ->
+  well_behaved_references m' t'.
+Proof.
+  intros * Htype Hwba Hwbr ?. inversion_mstep.
+  - clear Htype. clear Hwba.
+    induction_step; inversion Hwbr; subst;
+    eauto using well_behaved_references, wbr_subst.
+  - generalize dependent T. induction_step; intros * Htype;
+    try solve [
+      inversion Hwbr; inversion Htype;
+      destruct_wba; eauto using well_behaved_references, wbr_mem_add
+    ].
+    inversion_clear Htype; subst.
+    + eapply wbr_refM. rewrite (get_add_eq TM_Unit). trivial.
+    + eapply wbr_refI. rewrite (get_add_eq TM_Unit). trivial.
+  -
+      
+Qed.
+
+(* ------------------------------------------------------------------------- *)
+(* ------------------------------------------------------------------------- *)
+(* ------------------------------------------------------------------------- *)
 
 Lemma substitution_preservation : forall t tx T Tx Tx' Gamma x,
   Gamma |-- (TM_Fun x Tx t) is (TY_Fun Tx' T) ->
@@ -85,14 +151,8 @@ Proof.
   intros * ?. inversion_type. intros. eapply H; eauto.
 Qed.
 
-Definition memprop m m' :=
-  (forall ad T,
-  ad < length m ->
-  empty |-- (getTM m ad) is T ->
-  empty |-- (getTM m' ad) is T).
-
 Theorem preservation : forall m m' t t' eff T,
-  well_behaved_locations m t ->
+  well_behaved_references m t ->
   empty |-- t is T ->
   m / t ==[eff]==> m' / t' ->
   empty |-- t' is T.
@@ -107,6 +167,7 @@ Proof.
     eauto using well_typed_term.
     + inversion Htype; subst. shelve.
     + inversion Htype; subst. shelve.
-  - induction Htype; intros; inversion_step; eauto using well_typed_term.
+  - induction Htype; intros; inversion_step; try (inversion Hmem; subst);
+    eauto using well_typed_term.
 Qed.
 
